Source/IntegrationTests/TestFiles/LitTests/LitTest/comp/rust/newtypes.dfy
@@ -1,5 +1,5 @@
-// RUN: %baredafny run -t:rs --type-system-refresh --refresh-exit-code=0 "%s"
-// RUN: %baredafny run -t:rs --type-system-refresh --unicode-char=false --refresh-exit-code=0 "%s"
+// RUN: %baredafny run -t:rs "%s"
+// RUN: %baredafny run -t:rs --unicode-char=false "%s"
 /// RUN: %testDafnyForEachCompiler --refresh-exit-code=0 "%s"
 
 newtype int2 = x: int | -2 <= x < 2
@@ -67,16 +67,6 @@ newtype NestedIntWrapper = IntWrapper {
   }
 }
 
-newtype BoolWrapper = bool {
-  const n: int := if this then 1 else 0
-  static function True(): BoolWrapper {
-    true as BoolWrapper
-  }
-  function Or(other: BoolWrapper): BoolWrapper {
-    if n == 1 then True() else other
-  }
-}
-
 // Ensuring the uint32 is hashable
 datatype {:rust_rc false} UInt32Pair = UInt32Pair(first: uint32WithMethods, second: uint32WithMethods)
 
@@ -125,8 +115,4 @@ method Main(){
   expect 0 as uint32WithMethods == two.div_overflow(three);
   expect almost_overflow2 == almost_overflow.times_overflow(two);
   expect (3 as IntWrapper).DoublePlus(1 as IntWrapper) == 7 as IntWrapper;
-
-  expect (true as BoolWrapper).Or(false as BoolWrapper) == (true as BoolWrapper);
-  expect (false as BoolWrapper).Or(false as BoolWrapper) == (false as BoolWrapper);
-  expect (false as BoolWrapper).Or(true as BoolWrapper) == (true as BoolWrapper);  
 }
