Source/IntegrationTests/TestFiles/LitTests/LitTest/comp/rust/newtypesrefresh.dfy
@@ -1,0 +1,17 @@
+// RUN: %baredafny run -t:rs --type-system-refresh --general-newtypes "%s"
+
+newtype BoolWrapper = bool {
+  const n: int := if this then 1 else 0
+  static function True(): BoolWrapper {
+    true as BoolWrapper
+  }
+  function Or(other: BoolWrapper): BoolWrapper {
+    if n == 1 then True() else other
+  }
+}
+
+method Main(){
+  expect (true as BoolWrapper).Or(false as BoolWrapper) == (true as BoolWrapper);
+  expect (false as BoolWrapper).Or(false as BoolWrapper) == (false as BoolWrapper);
+  expect (false as BoolWrapper).Or(true as BoolWrapper) == (true as BoolWrapper);  
+}
